src/SoftBound/sb_pp.v
@@ -1,0 +1,408 @@
+Add LoadPath "../ssa/ott".
+Add LoadPath "../ssa/monads".
+Add LoadPath "../ssa/compcert".
+Add LoadPath "../ssa".
+Add LoadPath "../../../theory/metatheory_8.3".
+Add LoadPath "../TV".
+Require Import ssa_def.
+Require Import ssa_lib.
+Require Import List.
+Require Export targetdata.
+Require Import monad.
+Require Import Arith.
+Require Import Metatheory.
+Require Import genericvalues.
+Require Import trace.
+Require Import ssa_props.
+Require Import assoclist.
+Require Import sb_def.
+Require Import Coqlib.
+Require Import Memdata.
+Require Import Memory.
+Require Import Integers.
+Require Import sb_tactic.
+
+Import SoftBound.
+
+Definition wf_data (TD:TargetData) (M:mem) (gvb gve:GenericValue) : Prop :=
+  match (GV2ptr TD (getPointerSize TD) gvb,
+         GV2ptr TD (getPointerSize TD) gve) with
+  | (Some (Values.Vptr bb bofs), Some (Values.Vptr eb eofs)) =>
+      if zeq bb eb then
+        Mem.range_perm M bb (Int.signed 31 bofs) (Int.signed 31 eofs) Readable
+      else False
+  | _ => False
+  end.
+
+Definition wf_rmetadata (TD:TargetData) (M:mem) (rm:rmetadata) : Prop :=
+  forall (i:id) (gvb gve:GenericValue),
+    lookupAL _ rm i = Some (mkMD gvb gve) -> wf_data TD M gvb gve.
+
+Definition wf_mmetadata (TD:TargetData) (M:mem) (MM:mmetadata) : Prop :=
+  forall (b:Values.block) (ofs:int32) (gvb gve:GenericValue),
+    MM b ofs = Some (mkMD gvb gve) -> wf_data TD M gvb gve.
+
+Definition wf_metadata (TD:TargetData) (M:mem) (rm:rmetadata) (MM:mmetadata) 
+    : Prop :=
+  wf_rmetadata TD M rm /\ wf_mmetadata TD M MM.
+
+Lemma range_perm_alloc_other:
+  forall m1 lo hi m2 b, Mem.alloc m1 lo hi = (m2, b) ->
+  forall b' lo' hi' p,
+  Mem.range_perm m1 b' lo' hi' p ->
+  Mem.range_perm m2 b' lo' hi' p.
+Proof.
+  intros. inv H. red.
+Admitted.
+
+Lemma store_range_perm_1:
+  forall chunk m1 b ofs v m2, Mem.store chunk m1 b ofs v = Some m2 ->
+  forall b' lo' hi' p,
+  Mem.range_perm m1 b' lo' hi' p -> Mem.range_perm m2 b' lo' hi' p.
+Admitted.
+
+Lemma GV2ptr_base2GV : forall TD mb,
+  GV2ptr TD (getPointerSize TD) (base2GV TD mb) = 
+    Some (Values.Vptr mb (Int.repr 31 0)).
+Admitted.
+
+Lemma GV2ptr_bound2GV : forall TD mb tsz n,
+  GV2ptr TD (getPointerSize TD) (bound2GV TD mb tsz n) = 
+    Some (Values.Vptr mb (Int.repr 31 ((Size.to_Z tsz)*n))).
+Admitted.
+
+Lemma wf_mmetadata__wf_data : forall Mem0 TD MM b0 ofs gvb gve,
+  wf_mmetadata TD Mem0 MM ->
+  MM b0 ofs = Some (mkMD gvb gve) ->
+  wf_data TD Mem0 gvb gve.
+Proof.
+  intros Mem0 TD MM b0 ofs gvb gve Hwfm J.
+  apply Hwfm in J; clear Hwfm.
+  unfold wf_data in *.
+  destruct (GV2ptr TD (getPointerSize TD) gvb); auto.
+Qed.
+
+Lemma wf_data__store__wf_data : forall m Mem0 b ofs0 v0 Mem' TD gvb gve,
+  Mem.store m Mem0 b ofs0 v0 = Some Mem' ->
+  wf_data TD Mem0 gvb gve ->
+  wf_data TD Mem' gvb gve.
+Proof.
+  intros m Mem0 b ofs0 v0 Mem' TD gvb gve H1 J.
+  unfold wf_data in *.
+  destruct (GV2ptr TD (getPointerSize TD) gvb); auto.
+  destruct v; auto.
+  destruct (GV2ptr TD (getPointerSize TD) gve); auto.
+  destruct v; auto.
+  destruct (zeq b0 b1); eauto using store_range_perm_1.
+Qed.
+
+Lemma wf_mmetadata__store__wf_data : forall m Mem0 b ofs0 v0 Mem' TD MM b0 ofs 
+    gvb gve,
+  Mem.store m Mem0 b ofs0 v0 = Some Mem' ->
+  wf_mmetadata TD Mem0 MM ->
+  MM b0 ofs = Some (mkMD gvb gve) ->
+  wf_data TD Mem' gvb gve.
+Proof.
+  intros m Mem0 b ofs0 v0 Mem' TD MM b0 ofs gvb gve H1 Hwfm J.
+  apply wf_mmetadata__wf_data with (Mem0:=Mem0)(TD:=TD) in J; eauto.
+  eapply wf_data__store__wf_data; eauto.
+Qed.
+
+Lemma wf_rmetadata__get_reg_metadata : forall TD Mem0 rm gl vp gvb gve,
+  wf_rmetadata TD Mem0 rm ->
+  get_reg_metadata TD Mem0 gl rm vp = Some (mkMD gvb gve) ->
+  wf_data TD Mem0 gvb gve.
+Proof.
+  intros TD Mem0 rm gl vp gvb gve Hwfr J.
+  unfold get_reg_metadata in J.
+  destruct vp.
+    apply Hwfr in J; auto.
+
+    remember (get_const_metadata c) as R.
+    destruct R; try solve [inversion J].
+    destruct p.
+    remember (const2GV TD Mem0 gl c0) as R0.
+    remember (const2GV TD Mem0 gl c1) as R1.
+    destruct R0; try solve [inversion J]. simpl in J.
+    destruct R1; try solve [inversion J]. simpl in J.
+    inv J.
+    unfold wf_data.
+Admitted.
+
+Lemma dbCmd_preservation : forall TD lc rm als gl Mem MM c lc' rm' als' Mem' MM' 
+    tr r, 
+  dbCmd TD gl lc rm als Mem MM c lc' rm' als' Mem' MM' tr r ->
+  wf_metadata TD Mem rm MM ->
+  wf_metadata TD Mem' rm' MM'.
+Proof.
+  intros TD lc rm als gl Mem MM c lc' rm' als' Mem' MM' tr r H.
+  (sb_dbCmd_cases (destruct H) Case); intro Hwf; eauto.
+
+Case "dbMalloc".
+  invert_prop_reg_metadata. clear H3.
+  unfold malloc in H1.
+  rewrite H2 in H1.
+  remember (Mem.alloc Mem0 0 (Size.to_Z tsz * n)) as R.
+  inversion H1. clear H1. subst.
+  destruct Hwf as [Hwfr Hwfm].
+  split; auto.
+    clear H2 Hwfm. 
+    intros i0 gvb gve J.
+    destruct (@id_dec id0 i0); subst.
+      rewrite lookupAL_updateAddAL_eq in J.
+      inversion J; subst. clear J.
+      unfold wf_data.
+      rewrite GV2ptr_base2GV. 
+      rewrite GV2ptr_bound2GV. 
+      destruct (zeq mb mb) as [J | J]; try solve [contradict J; auto].
+      intros ofs J1. 
+(*
+      rewrite Int.signed_repr in J1; 
+        auto using Int.min_signed_neg, Int.max_signed_pos with zarith.
+*)
+      apply Mem.valid_access_alloc_same with (ofs:=ofs)(chunk:=AST.Mint 7) in H4.
+        destruct H4 as [J2 J3].
+        unfold Mem.range_perm in J2.
+        apply Mem.perm_implies with (p1:=Freeable); auto with mem.
+        apply J2.
+        simpl. unfold bytesize_chunk. admit.
+
+        admit. 
+        simpl. unfold bytesize_chunk. admit.
+        simpl. unfold bytesize_chunk. admit.
+      
+
+       rewrite <- lookupAL_updateAddAL_neq in J; auto.
+       assert (J':=@Hwfr i0 gvb gve J). clear Hwfr.    
+       unfold wf_data in *.
+       destruct (GV2ptr TD (getPointerSize TD) gvb); auto.
+       destruct v0; auto.
+       destruct (GV2ptr TD (getPointerSize TD) gve); auto.
+       destruct v0; auto.
+       destruct (zeq b b0); eauto using range_perm_alloc_other.
+
+    intros b ofs gvb gve J.
+    assert (J':=@Hwfm b ofs gvb gve J). clear Hwfm.
+    unfold wf_data in *.
+    destruct (GV2ptr TD (getPointerSize TD) gvb); auto.
+    destruct v0; auto.
+    destruct (GV2ptr TD (getPointerSize TD) gve); auto.
+    destruct v0; auto.
+    destruct (zeq b0 b1); eauto using range_perm_alloc_other.
+
+Case "dbFree".
+  admit.
+
+Case "dbAlloca".
+  invert_prop_reg_metadata. clear H3.
+  unfold malloc in H1.
+  rewrite H2 in H1.
+  remember (Mem.alloc Mem0 0 (Size.to_Z tsz * n)) as R.
+  inversion H1. clear H1. subst.
+  destruct Hwf as [Hwfr Hwfm].
+  split; auto.
+    clear H2 Hwfm. 
+    intros i0 gvb gve J.
+    destruct (@id_dec id0 i0); subst.
+      rewrite lookupAL_updateAddAL_eq in J.
+      inversion J; subst. clear J.
+      unfold wf_data in *.
+      rewrite GV2ptr_base2GV. 
+      rewrite GV2ptr_bound2GV. 
+      destruct (zeq mb mb) as [J | J]; try solve [contradict J; auto].
+      intros ofs J1. 
+(*
+      rewrite Int.signed_repr in J1; 
+        auto using Int.min_signed_neg, Int.max_signed_pos with zarith.
+*)
+      apply Mem.valid_access_alloc_same with (ofs:=ofs)(chunk:=AST.Mint 7) in H4.
+        destruct H4 as [J2 J3].
+        unfold Mem.range_perm in J2.
+        apply Mem.perm_implies with (p1:=Freeable); auto with mem.
+        apply J2.
+        simpl. unfold bytesize_chunk. admit.
+
+        admit. 
+        simpl. unfold bytesize_chunk. admit.
+        simpl. unfold bytesize_chunk. admit.
+      
+
+       rewrite <- lookupAL_updateAddAL_neq in J; auto.
+       assert (J':=@Hwfr i0 gvb gve J). clear Hwfr.    
+       unfold wf_data in *.
+       destruct (GV2ptr TD (getPointerSize TD) gvb); auto.
+       destruct v0; auto.
+       destruct (GV2ptr TD (getPointerSize TD) gve); auto.
+       destruct v0; auto.
+       destruct (zeq b b0); eauto using range_perm_alloc_other.
+
+    intros b ofs gvb gve J.
+    assert (J':=@Hwfm b ofs gvb gve J). clear Hwfm.
+    unfold wf_data in *.
+    destruct (GV2ptr TD (getPointerSize TD) gvb); auto.
+    destruct v0; auto.
+    destruct (GV2ptr TD (getPointerSize TD) gve); auto.
+    destruct v0; auto.
+    destruct (zeq b0 b1); eauto using range_perm_alloc_other.
+
+Case "dbLoad_ptr".
+  invert_prop_reg_metadata. clear H5.
+  destruct Hwf as [Hwfr Hwfm].
+  split; auto.
+    intros i0 gvb gve J.
+    destruct (@id_dec id0 i0); subst.
+      clear Hwfr.
+      rewrite lookupAL_updateAddAL_eq in J.
+      inversion J; subst. clear J.
+      unfold get_mem_metadata in H4.
+      remember (GV2ptr TD (getPointerSize TD) gvp) as R.
+      destruct R; try solve [inversion H4].
+      destruct v; try solve [inversion H4].
+      apply Hwfm in H4; auto.
+
+      clear Hwfm.
+      rewrite <- lookupAL_updateAddAL_neq in J; auto.
+      apply Hwfr in J; auto.
+
+Case "dbStore_nptr".
+  unfold mstore in H3.
+  destruct (GV2ptr TD (getPointerSize TD) gvp); try solve [inversion H3].
+  destruct v0; try solve [inversion H3].
+  destruct (typ2memory_chunk t); try solve [inversion H3].
+  destruct (GV2val TD gv); try solve [inversion H3].
+  destruct Hwf as [Hwfr Hwfm].
+  split.
+    clear Hwfm.
+    intros i1 gvb gve J.
+    apply Hwfr in J. clear Hwfr.
+    unfold wf_data in *.
+    destruct (GV2ptr TD (getPointerSize TD) gvb); auto.
+    destruct v1; auto.
+    destruct (GV2ptr TD (getPointerSize TD) gve); auto.
+    destruct v1; auto.
+    destruct (zeq b0 b1); eauto using store_range_perm_1.
+
+    clear Hwfr.
+    intros b0 ofs gvb gve J.
+    apply Hwfm in J. clear Hwfm.
+    unfold wf_data in *.
+    destruct (GV2ptr TD (getPointerSize TD) gvb); auto.
+    destruct v1; auto.
+    destruct (GV2ptr TD (getPointerSize TD) gve); auto.
+    destruct v1; auto.
+    destruct (zeq b1 b2); eauto using store_range_perm_1.
+
+Case "dbStore_ptr".
+  unfold mstore in H3.
+  destruct (GV2ptr TD (getPointerSize TD) gvp); try solve [inversion H3].
+  destruct v0; try solve [inversion H3].
+  destruct (typ2memory_chunk t); try solve [inversion H3].
+  destruct (GV2val TD gv); try solve [inversion H3].
+  destruct Hwf as [Hwfr Hwfm].
+  split.
+    clear Hwfm.
+    intros i1 gvb gve J.
+    apply Hwfr in J. clear Hwfr.
+    unfold wf_data in *.
+    destruct (GV2ptr TD (getPointerSize TD) gvb); auto.
+    destruct v1; auto.
+    destruct (GV2ptr TD (getPointerSize TD) gve); auto.
+    destruct v1; auto.
+    destruct (zeq b0 b1); eauto using store_range_perm_1.
+
+    intros b0 ofs gvb gve J. 
+    subst.
+    unfold set_mem_metadata in J.
+    destruct (GV2ptr TD (getPointerSize TD) gvp); 
+      try solve [eauto using wf_mmetadata__store__wf_data].
+    destruct v1; try solve [eauto using wf_mmetadata__store__wf_data].
+    destruct (zeq b0 b1); subst; 
+       simpl in J; eauto using wf_mmetadata__store__wf_data.
+    destruct (Int.eq_dec 31 i1 ofs); subst; 
+       simpl in J; eauto using wf_mmetadata__store__wf_data.
+  
+       inversion J; subst. clear J.
+       apply wf_rmetadata__get_reg_metadata in H5; auto.
+       eapply wf_data__store__wf_data; eauto.
+
+Case "dbGEP".
+  destruct Hwf as [Hwfr Hwfm].
+  split; auto.
+    clear Hwfm.
+    invert_prop_reg_metadata. clear H3.
+    intros i0 gvb gve J.
+    destruct (@id_dec id0 i0); subst.
+      rewrite lookupAL_updateAddAL_eq in J.
+      inversion J; subst. clear J.
+      eapply wf_rmetadata__get_reg_metadata; eauto.
+
+      rewrite <- lookupAL_updateAddAL_neq in J; auto.
+      apply Hwfr in J; auto.
+
+Case "dbBitcast_ptr".
+  destruct Hwf as [Hwfr Hwfm].
+  split; auto.
+    clear Hwfm.
+    invert_prop_reg_metadata. clear H2.
+    intros i0 gvb gve J.
+    destruct (@id_dec id0 i0); subst.
+      rewrite lookupAL_updateAddAL_eq in J.
+      inversion J; subst. clear J.
+      eapply wf_rmetadata__get_reg_metadata; eauto.
+
+      rewrite <- lookupAL_updateAddAL_neq in J; auto.
+      apply Hwfr in J; auto.
+
+Case "dbInttoptr".
+  destruct Hwf as [Hwfr Hwfm].
+  split; auto.
+    clear Hwfm.
+    invert_prop_reg_metadata. clear H0.
+    intros i0 gvb gve J.
+    destruct (@id_dec id0 i0); subst.
+      rewrite lookupAL_updateAddAL_eq in J.
+      inversion J; subst. clear J.
+      unfold wf_data.
+      simpl.
+      intros ofs J.
+      admit. (* J is false. *)
+
+      rewrite <- lookupAL_updateAddAL_neq in J; auto.
+      apply Hwfr in J; auto.
+
+Case "dbSelect_ptr".
+  destruct Hwf as [Hwfr Hwfm].
+  split; auto.
+    clear Hwfm.
+    destruct (isGVZero TD cond0). 
+      invert_prop_reg_metadata. clear H4.
+      intros i0 gvb gve J.
+      destruct (@id_dec id0 i0); subst.
+        rewrite lookupAL_updateAddAL_eq in J.
+        inversion J; subst. clear J.
+        eapply wf_rmetadata__get_reg_metadata; eauto.
+
+        rewrite <- lookupAL_updateAddAL_neq in J; auto.
+        apply Hwfr in J; auto.
+
+      invert_prop_reg_metadata. clear H4.
+      intros i0 gvb gve J.
+      destruct (@id_dec id0 i0); subst.
+        rewrite lookupAL_updateAddAL_eq in J.
+        inversion J; subst. clear J.
+        eapply wf_rmetadata__get_reg_metadata; eauto.
+
+        rewrite <- lookupAL_updateAddAL_neq in J; auto.
+        apply Hwfr in J; auto.
+
+Case "dbLib". admit.
+Case "dbLib_error". admit.
+Qed.
+
+(*****************************)
+(*
+*** Local Variables: ***
+*** coq-prog-name: "coqtop" ***
+*** coq-prog-args: ("-emacs-U" "-I" "~/SVN/sol/vol/src/ssa/monads" "-I" "~/SVN/sol/vol/src/ssa/ott" "-I" "~/SVN/sol/vol/src/ssa/compcert" "-I" "~/SVN/sol/theory/metatheory_8.3" "-I" "~/SVN/sol/vol/src/TV") ***
+*** End: ***
+ *)
