src/SoftBound/sb_tactic.v
@@ -1,0 +1,30 @@
+Add LoadPath "../ssa/ott".
+Add LoadPath "../ssa/monads".
+Add LoadPath "../ssa/compcert".
+Add LoadPath "../ssa".
+Add LoadPath "../../../theory/metatheory_8.3".
+Add LoadPath "../TV".
+Require Import sb_def.
+
+Ltac invert_prop_reg_metadata :=
+  match goal with
+  | [H : SoftBound.prop_reg_metadata _ _ _ _ _ = (_, _) |- _ ] =>
+      inversion H; subst; eauto
+  end.
+
+Ltac invert_result :=
+  match goal with
+  | [H : SoftBound.is_error SoftBound.rok |- _ ] => inversion H
+  | [H : SoftBound.rerror = SoftBound.rok |- _ ] => inversion H
+  | [H : SoftBound.rabort = SoftBound.rok |- _ ] => inversion H 
+  | [H : SoftBound.rok = SoftBound.rerror |- _ ] => inversion H 
+  | [H : SoftBound.rok = SoftBound.rabort |- _ ] => inversion H 
+ end.
+
+(*****************************)
+(*
+*** Local Variables: ***
+*** coq-prog-name: "coqtop" ***
+*** coq-prog-args: ("-emacs-U" "-I" "~/SVN/sol/vol/src/ssa/monads" "-I" "~/SVN/sol/vol/src/ssa/ott" "-I" "~/SVN/sol/vol/src/ssa/compcert" "-I" "~/SVN/sol/theory/metatheory_8.3" "-I" "~/SVN/sol/vol/src/TV") ***
+*** End: ***
+ *)
